Updates.

HandbookOfPracticalLogicLean/Chapter2/NF/CNF/ToCNF.lean
@@ -1,32 +1,13 @@
-import MathlibExtraLean.AllPairs
-
+import HandbookOfPracticalLogicLean.Chapter2.NF.DeMorgan
 import HandbookOfPracticalLogicLean.Chapter2.NF.NF
-import HandbookOfPracticalLogicLean.Chapter2.NF.Negate
 import HandbookOfPracticalLogicLean.Chapter2.NF.NNF.NNF_1
 import HandbookOfPracticalLogicLean.Chapter2.NF.DNF.ToDNF_3
-
-import HandbookOfPracticalLogicLean.Chapter2.NF.ListConj.Semantics
-import HandbookOfPracticalLogicLean.Chapter2.NF.ListDisj.Semantics
 
 
 set_option autoImplicit false
 
 
 open Formula_
-
-
-def map_map_not
-  (FSS : List (List Formula_)) :
-  List (List Formula_) :=
-  List.map (List.map not_) FSS
-
-#eval map_map_not ([[atom_ "P", atom_ "Q"], [atom_ "R", atom_ "S"]])
-
-
-def map_map_negate_literal
-  (FSS : List (List Formula_)) :
-  List (List Formula_) :=
-  List.map (List.map negate_literal) FSS
 
 
 /--
@@ -41,27 +22,6 @@ def to_cnf_v3_aux
 
 
 /--
-  Helper function for `to_cnf_v3`.
--/
-def to_cnf_v3_aux_alt :
-  Formula_ → List (List Formula_)
-  | and_ p q => (to_cnf_v3_aux_alt p) ∪ (to_cnf_v3_aux_alt q)
-  | or_ p q => all_pairs_v4 List.union (to_cnf_v3_aux_alt p) (to_cnf_v3_aux_alt q)
-  | F => [[F]]
-
-#eval (to_cnf_v3_aux_alt (Formula_| ((p \/ (q /\ r)) /\ (~ p \/ ~ r)))).toString
-
-
-/--
-  `list_of_lists_to_conjunction_of_disjunctions FSS` := Translates the list of lists of formulas `FSS` to a conjunction of disjunctions.
--/
-def list_of_lists_to_conjunction_of_disjunctions
-  (FSS : List (List Formula_)) :
-  Formula_ :=
-  list_conj (List.map list_disj FSS)
-
-
-/--
   `to_cnf_v3 F` := Translates the formula `F` to a logically equivalent formula. If `F` is in negation normal form then `to_cnf_v3 F` is in conjunctive normal form.
 -/
 def to_cnf_v3
@@ -71,224 +31,6 @@ def to_cnf_v3
 
 
 #eval (list_of_lists_to_conjunction_of_disjunctions [[atom_ "P", atom_ "Q"], [not_ (atom_ "P"), atom_ "R"]]).toString
-
-
-lemma de_morgan_1
-  (V : ValuationAsTotalFunction)
-  (P Q : Formula_) :
-  eval V (not_ (and_ P Q)) = true ↔
-    eval V (or_ (not_ P) (not_ Q)) = true :=
-  by
-  simp only [eval]
-  simp only [bool_iff_prop_or]
-  simp only [bool_iff_prop_not]
-  simp only [bool_iff_prop_and]
-  constructor
-  · intro a1
-    by_cases c1 : eval V P = true
-    case pos =>
-      right
-      intro contra
-      apply a1
-      exact ⟨c1, contra⟩
-    case neg =>
-      left
-      exact c1
-  · intro a1
-    intro contra
-    obtain ⟨contra_left, contra_right⟩ := contra
-    cases a1
-    case inl a1 =>
-      apply a1
-      exact contra_left
-    case inr a1 =>
-      apply a1
-      exact contra_right
-
-
-lemma de_morgan_2
-  (V : ValuationAsTotalFunction)
-  (P Q : Formula_) :
-  eval V (not_ (or_ P Q)) = true ↔
-    eval V (and_ (not_ P) (not_ Q)) = true :=
-  by
-  simp only [eval]
-  simp only [bool_iff_prop_and]
-  simp only [bool_iff_prop_not]
-  simp only [bool_iff_prop_or]
-  constructor
-  · intro a1
-    constructor
-    · intro contra
-      apply a1
-      left
-      exact contra
-    · intro contra
-      apply a1
-      right
-      exact contra
-  · intro a1 contra
-    obtain ⟨a1_left, a1_right⟩ := a1
-    cases contra
-    case inl contra =>
-      apply a1_left
-      exact contra
-    case inr contra =>
-      apply a1_right
-      exact contra
-
-
-lemma de_morgan_list_1
-  (V : ValuationAsTotalFunction)
-  (FS : List Formula_) :
-  eval V (not_ (list_conj FS)) = true ↔
-    eval V (list_disj (List.map not_ FS)) = true :=
-  by
-  induction FS
-  case nil =>
-    simp only [List.map_nil]
-    simp only [list_conj]
-    simp only [list_disj]
-    simp only [eval]
-    simp only [b_not]
-  case cons hd tl ih =>
-    cases tl
-    case nil =>
-      simp only [List.map_cons, List.map_nil]
-      unfold list_conj
-      unfold list_disj
-      rfl
-    case cons tl_hd tl_tl =>
-      simp only [List.map_cons] at ih
-
-      simp only [List.map_cons]
-      unfold list_conj
-      unfold list_disj
-      simp only [de_morgan_1]
-      unfold eval
-      simp only [bool_iff_prop_or]
-      rewrite [ih]
-      rfl
-
-
-lemma de_morgan_list_2
-  (V : ValuationAsTotalFunction)
-  (FS : List Formula_) :
-  eval V (not_ (list_disj FS)) = true ↔
-    eval V (list_conj (List.map not_ FS)) = true :=
-  by
-  induction FS
-  case nil =>
-    simp only [List.map_nil]
-    simp only [list_disj]
-    simp only [list_conj]
-    simp only [eval]
-    simp only [b_not]
-  case cons hd tl ih =>
-    cases tl
-    case nil =>
-      simp only [List.map_cons, List.map_nil]
-      unfold list_disj
-      unfold list_conj
-      rfl
-    case cons tl_hd tl_tl =>
-      simp only [List.map_cons] at ih
-
-      simp only [List.map_cons]
-      unfold list_disj
-      unfold list_conj
-      simp only [de_morgan_2]
-      unfold eval
-      simp only [bool_iff_prop_and]
-      rewrite [ih]
-      rfl
-
-
-lemma de_morgan_list_alt_1
-  (V : ValuationAsTotalFunction)
-  (FS : List Formula_) :
-  eval V (list_conj FS) = true ↔
-    eval V (not_ (list_disj (List.map not_ FS))) = true :=
-  by
-  simp only [eval]
-  simp only [bool_iff_prop_not]
-  rewrite [← de_morgan_list_1]
-  simp only [eval]
-  simp only [bool_iff_prop_not]
-  simp only [Bool.not_eq_true, Bool.not_eq_false]
-
-
-lemma de_morgan_list_alt_2
-  (V : ValuationAsTotalFunction)
-  (FS : List Formula_) :
-  eval V (list_disj FS) = true ↔
-    eval V (not_ (list_conj (List.map not_ FS))) = true :=
-  by
-  simp only [eval]
-  simp only [bool_iff_prop_not]
-  rewrite [← de_morgan_list_2]
-  simp only [eval]
-  simp only [bool_iff_prop_not]
-  simp only [Bool.not_eq_true, Bool.not_eq_false]
-
-
-lemma de_morgan_list_of_lists_1
-  (V : ValuationAsTotalFunction)
-  (FSS : List (List Formula_)) :
-  eval V (not_ (list_of_lists_to_disjunction_of_conjunctions FSS)) = true ↔
-    eval V (list_of_lists_to_conjunction_of_disjunctions (map_map_not FSS)) :=
-  by
-  unfold list_of_lists_to_disjunction_of_conjunctions
-  unfold list_of_lists_to_conjunction_of_disjunctions
-  unfold map_map_not
-  rewrite [de_morgan_list_2]
-  simp only [eval_list_conj_eq_true_iff_forall_eval_eq_true]
-  simp only [List.map_map, List.mem_map, Function.comp_apply]
-  constructor
-  · intro a1 F a2
-    obtain ⟨FS, a2_left, a2_right⟩ := a2
-    rewrite [← a2_right]
-    rewrite [← de_morgan_list_1]
-    apply a1
-    apply Exists.intro FS
-    constructor
-    · exact a2_left
-    · rfl
-  · intro a1 F a2
-    obtain ⟨FS, a2_left, a2_right⟩ := a2
-    rewrite [← a2_right]
-    rewrite [de_morgan_list_1]
-    apply a1
-    apply Exists.intro FS
-    constructor
-    · exact a2_left
-    · rfl
-
-
-lemma de_morgan_list_of_lists_2
-  (V : ValuationAsTotalFunction)
-  (FSS : List (List Formula_)) :
-  eval V (not_ (list_of_lists_to_conjunction_of_disjunctions FSS)) = true ↔
-    eval V (list_of_lists_to_disjunction_of_conjunctions (map_map_not FSS)) :=
-  by
-  unfold list_of_lists_to_conjunction_of_disjunctions
-  unfold list_of_lists_to_disjunction_of_conjunctions
-  unfold map_map_not
-  rewrite [de_morgan_list_1]
-  simp only [eval_list_disj_eq_true_iff_exists_eval_eq_true]
-  simp only [List.map_map, List.mem_map, Function.comp_apply]
-  simp only [exists_exists_and_eq_and]
-  constructor
-  · intro a1
-    obtain ⟨FS, a1_left, a1_right⟩ := a1
-    rewrite [de_morgan_list_2] at a1_right
-    apply Exists.intro FS
-    exact ⟨a1_left, a1_right⟩
-  · intro a1
-    obtain ⟨FS, a1_left, a1_right⟩ := a1
-    rewrite [← de_morgan_list_2] at a1_right
-    apply Exists.intro FS
-    exact ⟨a1_left, a1_right⟩
 
 
 lemma eval_eq_eval_to_cnf_v3
@@ -320,3 +62,6 @@ lemma list_of_lists_to_conjunction_of_disjunctions_singleton
   unfold list_disj
   unfold list_conj
   rfl
+
+
+#lint
