HandbookOfPracticalLogicLean/Chapter2/NF/ListOfListsTo.lean
@@ -1,0 +1,29 @@
+import HandbookOfPracticalLogicLean.Chapter2.NF.ListConj.ListConj
+import HandbookOfPracticalLogicLean.Chapter2.NF.ListDisj.ListDisj
+
+
+set_option autoImplicit false
+
+
+open Formula_
+
+
+/--
+  `list_of_lists_to_disjunction_of_conjunctions FSS` := Translates the list of lists of formulas `FSS` to a disjunction of conjunctions.
+-/
+def list_of_lists_to_disjunction_of_conjunctions
+  (FSS : List (List Formula_)) :
+  Formula_ :=
+  list_disj (List.map list_conj FSS)
+
+
+/--
+  `list_of_lists_to_conjunction_of_disjunctions FSS` := Translates the list of lists of formulas `FSS` to a conjunction of disjunctions.
+-/
+def list_of_lists_to_conjunction_of_disjunctions
+  (FSS : List (List Formula_)) :
+  Formula_ :=
+  list_conj (List.map list_disj FSS)
+
+
+#lint
